nola/examples/logic/proph_ag.v
@@ -1,0 +1,81 @@
+(** * Prophetic agreement *)
+
+From nola.examples.logic Require Import synty.
+From iris.bi Require Export fractional.
+From iris.base_logic.lib Require Export ghost_var.
+From iris.proofmode Require Import proofmode.
+
+(** Existential type over a syntactic type *)
+#[projections(primitive)]
+Record anyty := Anyty {
+  anyty_ty : nsynty;
+  anyty_val : anyty_ty;
+}.
+Add Printing Constructor anyty.
+
+(** Ghost state *)
+Class proph_agG Σ := proph_agG_in :: ghost_varG Σ anyty.
+Definition proph_agΣ := ghost_varΣ anyty.
+#[export] Instance subG_proph_agΣ `{!subG proph_agΣ Σ} : proph_agG Σ.
+Proof. solve_inG. Qed.
+
+Section proph_ag.
+  Context `{!proph_agG Σ, !prophGS nsynty Σ}.
+
+  (** Value observer *)
+  Definition vo γ X x : iProp Σ := (ghost_var γ (1/2) (Anyty X x)).
+  (** Double value observer *)
+  Definition vo2 γ X x : iProp Σ := (ghost_var γ 1 (Anyty X x)).
+  (** Prophecy controller *)
+  Definition pc γ X x (ξ : prvar X) : iProp Σ :=
+    (vo γ X x ∗ 1:[ξ]) ∨
+    ((∃ x', vo2 γ X x') ∗ ⟨π, π ξ = x⟩).
+
+  (** [vo] and [vo2] can't coexist *)
+  Lemma vo_vo2 {γ X x x'} : vo γ X x -∗ vo2 γ X x' -∗ False.
+  Proof.
+    iIntros "vo vo'". by iDestruct (ghost_var_valid_2 with "vo vo'") as %[? _].
+  Qed.
+
+  (** Allocate [vo] and [pc] *)
+  Lemma vo_pc_alloc {X x} {ξ : prvar X} : 1:[ξ] ==∗ ∃ γ, vo γ X x ∗ pc γ X x ξ.
+  Proof.
+    iIntros "ξ". iMod ghost_var_alloc as (γ) "[vo vo']". iModIntro. iExists _.
+    iFrame "vo". iLeft. iFrame.
+  Qed.
+
+  (** Agreement between [vo] and [pc] *)
+  Lemma vo_pc_agree {γ X x x' ξ} : vo γ X x -∗ pc γ X x' ξ -∗ ⌜x = x'⌝.
+  Proof.
+    iIntros "vo [[vo' _]|[[% vo2] _]]"; last first.
+    { iDestruct (vo_vo2 with "vo vo2") as %[]. }
+    iDestruct (ghost_var_agree with "vo vo'") as %?. by simplify_eq.
+  Qed.
+
+  (** Update the value of [vo] and [pc] *)
+  Lemma vo_pc_update {γ X x x' y ξ} :
+    vo γ X x -∗ pc γ X x' ξ ==∗ vo γ X y ∗ pc γ X y ξ.
+  Proof.
+    iIntros "vo [[vo' ξ]|[[% vo2] _]]"; last first.
+    { iDestruct (vo_vo2 with "vo vo2") as %[]. }
+    iMod (ghost_var_update_2 with "vo vo'") as "[$ vo]"; [by rewrite Qp.div_2|].
+    iModIntro. iLeft. iFrame.
+  Qed.
+
+  (** Resolve the prophecy of [pc] *)
+  Lemma vo_pc_preresolve {γ X x x'} ξ aπ ηl q : aπ ./ ηl →
+    q:∗[ηl] -∗ vo γ X x -∗ pc γ X x' ξ =[proph_wsat]=∗
+      q:∗[ηl] ∗ ⟨π, π ξ = aπ π⟩ ∗ (∀ y, ⟨π, aπ π = y⟩ -∗ pc γ X y ξ).
+  Proof.
+    iIntros "% ηl vo [[vo' ξ]|[[% vo2] _]]"; last first.
+    { iDestruct (vo_vo2 with "vo vo2") as %[]. }
+    iMod (proph_resolve_dep with "ξ ηl") as "[$ #obs]"; [done|]. iModIntro.
+    iFrame "obs". iIntros "%y obs'". iRight. iCombine "vo vo'" as "vo2".
+    iSplit; [by iExists _|]. by iApply (proph_obs_impl2 with "obs obs'")=> ?->.
+  Qed.
+  Lemma pc_resolve {γ X x} ξ :
+    pc γ X x ξ =[proph_wsat]=∗ ⟨π, π ξ = x⟩.
+  Proof.
+    iIntros "[[_ ξ]|[_ $]]"; [|done]. iApply (proph_resolve with "ξ").
+  Qed.
+End proph_ag.
